new-backend/bvpScript.sml
@@ -2,7 +2,7 @@ open HolKernel Parse boolLib bossLib; val _ = new_theory "bvp";
 
 open pred_setTheory arithmeticTheory pairTheory listTheory combinTheory;
 open finite_mapTheory sumTheory relationTheory stringTheory optionTheory;
-open bytecodeTheory bvlTheory sptreeTheory lcsymtacs bviTheory;
+open bvlTheory sptreeTheory lcsymtacs bviTheory;
 
 infix \\ val op \\ = op THEN;
 
